proov that well-formed commands can perform well

language_formal/spark2014_semantics/propertyProof.v
@@ -13,76 +13,147 @@ Inductive symbol_consistent: stack -> symtb -> Prop :=
                           (forall v, (Some v = fetch x s) -> stored_value_type (Value v) t)) -> 
         symbol_consistent s tb.
 
-Axiom eval_type_reserve: 
+(*
+Inductive return_value_type : return_val -> typ -> Prop :=
+    EVT_Int : forall n : Z, return_value_type (ValNormal (Int n)) Tint
+  | EVT_Bool : forall b : bool, return_value_type (ValNormal (Bool b)) Tbool
+
+Inductive stored_value_type : val -> typ -> Prop :=
+    SVT_Int : forall n : Z, stored_value_type (Value (Int n)) Tint
+  | SVT_Bool : forall b : bool, stored_value_type (Value (Bool b)) Tbool
+
+*)
+
+Ltac rm_contradict := 
+    match goal with
+    | [h: return_value_type ValException Tint |- _ ] =>  inversion h
+    | [h: return_value_type ValException Tbool |- _ ] =>  inversion h
+    | [h: return_value_type (ValNormal (Bool _)) Tint |- _ ] =>  inversion h
+    | [h: return_value_type (ValNormal (Int _)) Tbool |- _ ] =>  inversion h
+    | [h: Some ?T = binop_type ?OP Tint Tbool |- _ ] => unfold binop_type in h; simpl in h; inversion h
+    | [h: Some ?T = binop_type ?OP Tbool Tint |- _ ] => unfold binop_type in h; simpl in h; inversion h
+    end.
+
+Ltac rm_contradict2 :=
+    match goal with
+    | [h: return_value_type ValException ?t |- _] => destruct t; inversion h
+    end.
+
+Lemma eval_type_reserve: 
     forall (s: stack) (tb: symtb) e v t,
     symbol_consistent s tb -> 
     eval_expr s e v ->
     well_typed_expr tb e t ->
-    return_value_type v t. 
+    return_value_type v t.
+Proof.
+    intros s tb e.
+    induction e;
+    intros v t h1 h2 h3;
+    inversion h3;
+    inversion h2; subst. 
+  - (* Econst *)
+    constructor.
+  - constructor.  
+  - (* Evar *)
+    inversion h1; subst.
+    symmetry in H3.
+    specialize (H0 i In t H3).
+    rm_exists.
+    specialize (H2 _ H8).
+    apply value_type_consistent; assumption.
+  - (* Ebinop *)
+    specialize (IHe1 v1 t0 h1 H14 H5).
+    specialize (IHe2 v2 t0 h1 H15 H6).
+    destruct v1 as [v11 | v12]; try rm_contradict2.
+    destruct v2 as [v21 | v22]; try rm_contradict2.
+    destruct v11; destruct v21;
+    destruct t0; try rm_contradict.
+    + destruct b; repeat simpl_binop_hyp;
+       try constructor.
+    + destruct b; try simpl_binop_hyp;
+       constructor.
+  - (* Eunop *)
+    unfold eval_unop; destruct op; simpl.
+    constructor.
+Qed.
 
 (* basic lemmas *)
-Lemma binop_ind: forall s tb ast_id op e1 e2 v1 v2 t,
-    eval_expr s e1 (ValNormal (Int v1)) ->
-    eval_expr s e2 (ValNormal (Int v2)) -> 
-    well_typed_expr tb (Ebinop ast_id op e1 e2) t -> (* for example, disallow expression: 8 /\ 9 *)
+Ltac br_rm_rop v1 v2 op v1' v2' :=
+    match goal with
+    | [ |- exists v : value, eval_expr _ (Ebinop ?ast_id ?rop ?e1 ?e2) (ValNormal ?v)] =>
+            assert (exists b, ValNormal (Bool b) = eval_binop rop (ValNormal v1) (ValNormal v2))
+    end; [ simpl_binop; exists (op v1' v2'); auto | ].
+
+Ltac br_rm_aop v1 v2 v3 :=
+    match goal with
+    | [ |- exists v : value, eval_expr _ (Ebinop ?ast_id ?aop ?e1 ?e2) (ValNormal ?v)] =>
+            assert (exists n, ValNormal (Int n) = eval_binop aop (ValNormal v1) (ValNormal v2))
+    end; [ simpl_binop; exists v3; auto | ].
+
+Ltac br_clearer v f :=
+    exists v;
+    rm_eval_expr; unfold f; auto.   
+
+Lemma binop_rule: forall s tb e1 v1 e2 v2 ast_id op t,
     symbol_consistent s tb -> 
-    (exists v : Z, eval_expr s (Ebinop ast_id op e1 e2) (ValNormal (Int v))) \/ 
-    (exists b: bool, eval_expr s (Ebinop ast_id op e1 e2) (ValNormal (Bool b))).
+    eval_expr s e1 (ValNormal v1) ->
+    eval_expr s e2 (ValNormal v2) -> 
+    well_typed_expr tb (Ebinop ast_id op e1 e2) t -> (* for example, disallow expression: 8 /\ 9 *)
+    (exists v : value, eval_expr s (Ebinop ast_id op e1 e2) (ValNormal v)).
+Proof.    
+    intros.
+    inversion H2; subst.
+    specialize (eval_type_reserve s tb e1 (ValNormal v1) t0 H H0 H9); intros h1.
+    specialize (eval_type_reserve s tb e2 (ValNormal v2) t0 H H1 H10); intros h2.    
+    destruct v1 as [v11 | v12]; destruct v2 as [v21 | v22]; 
+    inversion h1; subst; try rm_contradict. 
+  - (* Ebinop Tint Tint *)
+    destruct op; try simpl_binop_hyp;
+    [ br_rm_rop (Int v11) (Int v21) Zeq_bool v11 v21 |
+      br_rm_rop (Int v11) (Int v21) Zneq_bool v11 v21 |
+      br_rm_aop (Int v11) (Int v21) (v11 + v21)%Z |
+      br_rm_aop (Int v11) (Int v21) (v11 - v21)%Z |
+      br_rm_aop (Int v11) (Int v21) (v11 * v21)%Z |
+      br_rm_aop (Int v11) (Int v21) (v11 / v21)%Z
+    ]; rm_exists;
+    [br_clearer (Bool x) good_value | br_clearer (Bool x) good_value | | | | ];
+    br_clearer (Int x) good_value.
+  - (* Ebinop Tbool Tbool *)
+    destruct op; 
+    simpl; 
+    try simpl_binop_hyp.
+    br_clearer (Bool (v12 && v22)) eval_binop.    
+    br_clearer (Bool (v12 || v22)) eval_binop.   
+Qed.
+
+Ltac ru_rm_unop v1 v2 :=
+    match goal with
+    [ |- exists b : value, eval_expr _ (Eunop ?ast_id ?uop ?e) (ValNormal b)] => 
+            assert (exists b, ValNormal (Bool b) = eval_unop uop (ValNormal v1)) 
+    end; 
+    [simpl_unop; exists v2; auto | ].
+
+Ltac ur_clearer v :=
+    exists v;
+    eapply eval_Eunop; eassumption.   
+
+Lemma unop_rule: forall s tb e v ast_id op t,
+    symbol_consistent s tb -> 
+    eval_expr s e (ValNormal v) ->
+    well_typed_expr tb (Eunop ast_id op e) t -> 
+    (exists bv : value, eval_expr s (Eunop ast_id op e) (ValNormal bv)).
 Proof.
     intros.
     inversion H1; subst.
-    specialize (eval_type_reserve s tb e1 (ValNormal (Int v1)) t0 H2 H H9); intros.
-    specialize (eval_type_reserve s tb e2 (ValNormal (Int v2)) t0 H2 H0 H10); intros.
-    inversion H3; subst.
-    (* destruct on the binary operator *)
-    destruct op; simpl;
-    (* 1. Oand | Oor *)
-    [right | right | inversion H11 | inversion H11 | left | left | left | left];
-    [(* 2. Ceq *)
-     assert (exists b, ValNormal (Bool b) = eval_binop Ceq (ValNormal (Int v1)) (ValNormal (Int v2))); 
-         [simpl_binop; exists (Zeq_bool v1 v2); auto | ] |
-     (* 3. Cne *)
-     assert (exists b, ValNormal (Bool b) = eval_binop Cne (ValNormal (Int v1)) (ValNormal (Int v2))); 
-          [simpl_binop; exists (Zneq_bool v1 v2); auto | ] |
-     (* 4. Oadd *)
-     assert (exists n, ValNormal (Int n) = eval_binop Oadd (ValNormal (Int v1)) (ValNormal (Int v2))); 
-         [simpl_binop; exists (v1 + v2)%Z; auto | ] |
-     (* 5. Osub *)
-     assert (exists n, ValNormal (Int n) = eval_binop Osub (ValNormal (Int v1)) (ValNormal (Int v2))); 
-         [simpl_binop; exists (v1 - v2)%Z; auto | ] |
-     (* 6. Oml *)
-     assert (exists n, ValNormal (Int n) = eval_binop Omul (ValNormal (Int v1)) (ValNormal (Int v2))); 
-         [simpl_binop; exists (v1 * v2)%Z; auto | ] |
-     (* 7. Odiv *)
-     assert (exists n, ValNormal (Int n) = eval_binop Odiv (ValNormal (Int v1)) (ValNormal (Int v2)));
-         [simpl_binop; exists (v1 / v2)%Z; auto | ]
-    ];
-    inversion H5; exists x;
-    rm_eval_expr; unfold good_value; auto.
-Qed.
+    specialize (eval_type_reserve s tb e (ValNormal v) Tbool H H0 H6); 
+    intros h1.
+    destruct v; try rm_contradict.
+    destruct op.
+    ru_rm_unop (Bool b) (negb b).
+    rm_exists.  
+    ur_clearer (Bool x).
+Qed. 
 
-Lemma binop_ind': forall s tb ast_id op e1 e2 v1 v2 t,
-    eval_expr s e1 (ValNormal (Bool v1)) ->
-    eval_expr s e2 (ValNormal (Bool v2)) -> 
-    well_typed_expr tb (Ebinop ast_id op e1 e2) t -> (* for example, disallow expression: 8 and 9 *)
-    symbol_consistent s tb -> 
-    (exists b: bool, eval_expr s (Ebinop ast_id op e1 e2) (ValNormal (Bool b))).
-Proof.
-    intros. 
-    inversion H1; subst.
-    specialize (eval_type_reserve s tb e1 (ValNormal (Bool v1)) t0 H2 H H9). intros.
-    specialize (eval_type_reserve s tb e2 (ValNormal (Bool v2)) t0 H2 H0 H10). intros.
-    inversion H3; subst.
-    assert (exists b, ValNormal (Bool b) = eval_binop op (ValNormal (Bool v1)) (ValNormal (Bool v2))).
-    unfold eval_binop. 
-    destruct op; simpl; try (inversion H11).
-    exists (v1 && v2). auto.
-    exists (v1 || v2). auto.
-    inversion H5. 
-    exists x. 
-    rm_eval_expr.
-Qed.
-    
 Theorem well_formed_expr: forall tb s e t,
     well_typed_expr tb e t ->
     well_defined_expr s e ->
@@ -117,8 +188,12 @@ Proof.
     destruct IHe1; destruct IHe2.
     * (* 3.1 ValInt, ValInt *)
       inversion H2. inversion H3.
-      specialize (binop_ind s tb a b e1 e2 x x0 t H4 H6 H H1). 
-      intros. apply H7.
+
+      specialize (binop_rule s tb e1 (Int x) e2 (Int x0) a b t H1 H4 H6 H).
+      intros h1. inversion h1. destruct x1 as [x2 | x3]. 
+      left; exists x2; assumption.
+      right; exists x3; assumption.
+
     * (* 3.2 ValInt, ValBool *)
       inversion H2. inversion H3.
       specialize (eval_type_reserve s tb e1 (ValNormal (Int x)) t0 H1 H4 H8); intros.
@@ -131,203 +206,183 @@ Proof.
       inversion H7; subst. inversion H12.
     * (* 3.4 ValBool, ValBool *)
       inversion H2. inversion H3.
+
+      specialize (binop_rule s tb e1 (Bool x) e2 (Bool x0) a b t H1 H4 H6 H).
+      intros h2. inversion h2. destruct x1 as [x2 | x3]. 
+      left; exists x2; assumption.
+      right; exists x3; assumption.
+(*      
       specialize (binop_ind' s tb a b e1 e2 x x0 t H4 H6 H H1). 
       intros. right; apply H7.
+*)
   - (* 4. Eunop *)
     inversion H; subst. 
     inversion H0; subst.
     specialize (IHe Tbool H6 H4 H1). 
-    inversion IHe; inversion H2.
-    * (* 4.1 ValInt *)
-      left. 
-      inversion H; subst.
-      specialize (eval_type_reserve s tb e (ValNormal (Int x)) Tbool H1 H3 H8); intros. 
-      inversion H5.
-    * (* 4.2 ValBool *)
-      right. 
-      assert (exists b, ValNormal (Bool b) = eval_unop u (ValNormal (Bool x))).
-      unfold eval_unop. destruct u. simpl. exists (negb x). auto.
-      inversion H5; subst. exists x0. 
-      eapply eval_Eunop; eassumption.
+    inversion IHe; rm_exists.    
+    + specialize (eval_type_reserve s tb e (ValNormal (Int x)) Tbool H1 H3 H6); 
+       intros h3; 
+       inversion h3. 
+    + specialize (unop_rule s tb e (Bool x) a u Tbool H1 H3 H); 
+       intros h4; inversion h4. 
+       destruct x0 as [x2 | x3]. 
+       left; exists x2; assumption.
+       right; exists x3; assumption.
 Qed.
 
-(* -> : this direction doesn't work *)
-(*
-Theorem well_formed_stmt: forall tb s c,
+(* = = = = = = = = = = = = = = =  *)
+(* = = = = = = = = = = = = = = =  *)
+
+Axiom valid_update: forall s tb ast_id x e v,
+    symbol_consistent s tb ->
+    well_typed_stmt tb (Sassign ast_id x e) ->
+    exists s', update s x (Value v) = Some s'.
+
+(* -> *)
+Axiom equal_wd_expr_expr2_R: forall s istate e,  
+    initializationMap s istate ->
+    well_defined_expr s e -> 
+    well_defined_expr2 istate e.
+
+(* <- *)    
+Axiom equal_wd_expr_expr2_L: forall s istate e,
+    initializationMap s istate ->
+    well_defined_expr2 istate e -> 
+    well_defined_expr s e.
+
+Axiom symbol_consistent_reserve: forall s tb k c s',
+     symbol_consistent s tb -> 
+     f_eval_stmt k s c = SNormal s' -> 
+     symbol_consistent s' tb.
+
+Axiom imap_exists: forall s, exists istate, 
+    initializationMap s istate.
+
+Axiom initializationMap_consistent: forall (s: stack) istate k s c1 s' istate' c2 istate'' istate1,
+     initializationMap s istate ->
+     f_eval_stmt k s c1 = SNormal s' -> 
+     well_defined_stmt2 istate c1 istate' -> 
+     well_defined_stmt2 istate' c2 istate'' ->      
+     initializationMap s' istate1 ->
+     exists istate2, well_defined_stmt2 istate1 c2 istate2. 
+
+Axiom type_consistent: forall s tb b v, 
+    symbol_consistent s tb ->
+    well_typed_expr tb b Tbool ->
+    ~eval_expr s b (ValNormal (Int v)).  
+
+Axiom initializationMap_Expr: forall (s: stack) istate e k c s' istate',
+    initializationMap s istate ->
+    well_defined_expr2 istate e ->
+    f_eval_stmt k s c = SNormal s' ->
+    initializationMap s' istate' ->
+    well_defined_expr2 istate' e.
+
+Axiom initializationMap_Stmt: forall (s: stack) istate k c s' istate' istate1,
+    initializationMap s istate ->
+    f_eval_stmt k s c = SNormal s' ->
+    well_defined_stmt2 istate c istate' ->
+    initializationMap s' istate1 ->
+    exists istate2, well_defined_stmt2 istate1 c istate2.
+
+
+(* Lemmas to prove... *)
+Lemma well_formed_cmd: forall k s tb c istate istate', 
+    symbol_consistent s tb ->
+    initializationMap s istate ->
     well_typed_stmt tb c ->
-    well_defined_stmt s c ->
-    symbol_consistent s tb -> 
-    exists s1, eval_stmt_R s c s1.
-*)
-
-(*
-Theorem good_expr_props: forall tb s e v n b,
-    symbol_consistent s tb /\ eval_expr s e v /\ (v = (ValNormal (Int n)) \/ v = (ValNormal (Bool b))) ->
-        (exists t, well_typed_expr tb e t) /\ well_defined_expr s e.
+    well_defined_stmt2 istate c istate' ->
+    (exists s', f_eval_stmt k s c = (SNormal s')) \/ f_eval_stmt k s c = SUnterminated.
 Proof.
-    intros tb s.
-    induction e; 
-    intros v n b0 H;
-    destruct H as [h [h1 h2]].
-  - (* 1. Econst *)
-    split.
-    + (* well_typed *)
-      destruct c.
-      * exists Tint; constructor.
-      * exists Tbool; constructor.
-    + (* well_defined *)
-      rm_wd_expr. 
-  - (* 2. Evar *)
-    split.
-    + (* well_typed *)
-       inversion h; subst.
-       inversion h2; subst; (* split into two cases: *) 
-       inversion h1; subst;
-       [specialize (H i (Int n) H3) | 
-        specialize (H i (Bool b0) H3)];
-       inversion H; clear H. 
-       inversion H1. exists x. (* made some modification from here to next '+' *)
-       rm_wt_expr. 
-       rm_exists.
-       exists x; rm_wt_expr.
-       inversion H1;
-       exists x; rm_wt_expr; 
+    intros k s tb c. 
+    functional induction (f_eval_stmt k s c);
+    intros istate istate' h1 h2 h3 h4;
+    try intuition.
+  - left.
+    exists s1. auto.
+  - left. 
+    (**)specialize (valid_update s tb ast_id x e0 v h1 h3). intros h5.
+    inversion h5; subst.
+    rewrite e3 in H. inversion H.
+  - inversion h4; subst.
+    inversion h3; subst.
+    (**)specialize (equal_wd_expr_expr2_L s istate e0 h2 H4). intros h6.
+    specialize (well_formed_expr tb s e0 t H6 h6 h1). intros.
+    inversion H; inversion H0.
+    + specialize (f_eval_expr_complete s e0 (ValNormal (Int x0)) H1). intros h7.
+       rewrite e2 in h7. inversion h7.
+    + specialize (f_eval_expr_complete s e0 (ValNormal (Bool x0)) H1). intros h7.
+       rewrite e2 in h7. inversion h7.
+  - (* Cseq *) 
+    inversion h3; subst.
+    inversion h4; subst.
+    specialize (IHs0 istate s' h1 h2 H2 H6).
+    (**)specialize (symbol_consistent_reserve s tb k' c1 s1 h1 e1). intros h8.
+    specialize (imap_exists s1). intros h9. inversion h9; clear h9.
+
+    (**)specialize (initializationMap_consistent s istate k' s c1 s1 s' c2 istate' x h2 e1 H6 H7 H). intros h9.
+    inversion h9.    
+    specialize (IHs1 x x0 h8 H H4 H0). assumption.    
+    
+  - inversion h3; subst. inversion h4; subst.
+    specialize (IHs0 istate s' h1 h2 H2 H6).
+    inversion IHs0.
+    + inversion H. rewrite e1 in H0; inversion H0.
+    + rewrite e1 in H; inversion H.
+  - (* Cifthen *)
+    inversion h3; subst.
+    inversion h4; subst.
+    specialize (IHs0 istate' s' h1 h2 H4 H7). assumption.
+  - left. exists s; auto.  
+  - inversion h3; subst.
+    inversion h4; subst.
+    (**)specialize (equal_wd_expr_expr2_L s istate' b h2 H6). intros h6.
+    (**)specialize (well_formed_expr tb s b Tbool H2 h6 h1). intros h7.
+    inversion h7.
+    + inversion H.
+       specialize (type_consistent s tb b x h1 H2). intros h8.
        intuition.
-    + (* well_defined *)
-      destruct h2; subst; 
-      inversion h1; subst;
-      rm_wd_expr.
-  - (* 3. Ebinop *)
-    split.
-    + (* well_typed *)
-       inversion h1; subst. 
-       inversion h2 as [h3 | h4]; clear h2. (* --> split into two cases: *)
-       (* Int case *)
-       specialize (expr_type_infer b v1 v2 n h3); intros H1.
-       rm_exists.
-       subst v1 v2.
-       specialize (IHe1 (ValNormal (Int x)) x true).
+    + inversion H.
+       apply f_eval_expr_complete in H0. 
+       rewrite H0 in y.
+       destruct x in y; intuition.
+  - (* Swhile *)
+    inversion h3; subst.
+    inversion h4; subst.
+    specialize (IHs0 istate' s' h1 h2 H4 H7).
+    (**)specialize (symbol_consistent_reserve s tb k' c0 s1 h1 e2). intros h8.
+    specialize (imap_exists s1). intros h9. inversion h9; clear h9.
+    
+    assert(well_defined_stmt2 x (Swhile ast_id b c0) x).
+    (**)specialize (initializationMap_Expr s istate' b k' c0 s1 x   h2 H6 e2 H). intros h9.
+    assert(exists y, well_defined_stmt2 x c0 y).
+    (**)specialize (initializationMap_Stmt s istate' k' c0 s1 s' x h2 e2 H7 H). intros h10.
+    inversion h10; clear h10.
+    exists x0; assumption.
+    inversion H0.
+    apply WD_Swhile2 with (s' := x0); assumption.
+    
+    specialize (IHs1 x x h8 H h3 H0).
+    assumption.
+  - inversion h3; subst.
+    inversion h4; subst.
+    specialize (IHs0 istate' s' h1 h2 H4 H7). 
+    inversion IHs0.
+    + inversion H. rewrite e2 in H0; inversion H0.
+    + rewrite e2 in H; inversion H.
+  - left. exists s; auto.
+  -  inversion h3; subst.
+    inversion h4; subst.
+    (**)specialize (equal_wd_expr_expr2_L s istate' b h2 H6). intros h6.
+    (**)specialize (well_formed_expr tb s b Tbool H2 h6 h1). intros h7.
+    inversion h7.
+    + inversion H.
+       specialize (type_consistent s tb b x h1 H2). intros h8.
        intuition.
-       specialize (IHe2 (ValNormal (Int x0)) x0 true).
-       intuition.
-       rm_exists.
-       specialize (eval_type_reserve s tb e1 (ValNormal (Int x)) x2 h H5 H0); intros H8.
-       specialize (eval_type_reserve s tb e2 (ValNormal (Int x0)) x1 h H6 H3); intros H9.       
-       inversion H8; clear H8; subst. inversion H9; clear H9; subst.
-       unfold eval_binop in h3. 
-       destruct b; try (inversion h3).
-           exists Tint; rm_wt_expr. 
-           exists Tint; rm_wt_expr.
-           exists Tint; rm_wt_expr.
-           exists Tint; rm_wt_expr.
-       (* Bool case *)
-       specialize (expr_type_infer' b v1 v2 b0 h4); intros H1.
-       inversion H1; clear H1; 
-       rm_exists; subst.
-       specialize (IHe1 (ValNormal (Int x)) x true).
-       intuition.
-       specialize (IHe2 (ValNormal (Int x0)) x0 true).
-       intuition.
-       rm_exists.
-       specialize (eval_type_reserve s tb e1 (ValNormal (Int x)) x2 h H5 H0); intros H8.
-       specialize (eval_type_reserve s tb e2 (ValNormal (Int x0)) x1 h H6 H3); intros H9.       
-       inversion H8; clear H8; subst. inversion H9; clear H9; subst.
-       unfold eval_binop in h4. 
-       destruct b; try (inversion h4).
-           exists Tbool; rm_wt_expr. 
-           exists Tbool; rm_wt_expr.
-       (***)
-       specialize (IHe1 (ValNormal (Bool x)) 0%Z x).
-       intuition.
-       specialize (IHe2 (ValNormal (Bool x0)) 0%Z x0).
-       intuition.
-       rm_exists.
-       specialize (eval_type_reserve s tb e1 (ValNormal (Bool x)) x2 h H5 H4); intros H8.
-       specialize (eval_type_reserve s tb e2 (ValNormal (Bool x0)) x1 h H6 H3); intros H9.       
-       inversion H8; clear H8; subst. inversion H9; clear H9; subst.
-       unfold eval_binop in h4. 
-       destruct b; try (inversion h4).
-           exists Tbool; rm_wt_expr. 
-           exists Tbool; rm_wt_expr.
-    + (* well_defined *)
-       inversion h2; clear h2; subst.
-       inversion h1; subst. 
-       symmetry in H7.
-       specialize (expr_type_infer b v1 v2 n H7); intros H1.
-       rm_exists. subst.
-       specialize (IHe1 (ValNormal (Int x)) x true).
-       intuition.
-       specialize (IHe2 (ValNormal (Int x0)) x0 true).
-       intuition.
-       rm_exists.
-       rm_wd_expr.
-       (**)
-       inversion h1; subst.
-       symmetry in H7.
-       specialize (expr_type_infer' b v1 v2 b0 H7); intros H1.
-       inversion H1.
-       rm_exists. subst.
-       clear H1.
-       specialize (IHe1 (ValNormal (Int x)) x true).
-       intuition.
-       specialize (IHe2 (ValNormal (Int x0)) x0 true).
-       intuition. rm_wd_expr.
-       rm_exists. subst.
-       clear H1.
-       specialize (IHe1 (ValNormal (Bool x)) 0%Z x).
-       intuition.
-       specialize (IHe2 (ValNormal (Bool x0)) 0%Z x0).
-       intuition. rm_wd_expr.
-  - (* 4. Eunop *)
-    split.
-    + (* well_typed *)
-       inversion h2; clear h2; subst.
-       inversion h1; subst.
-       unfold eval_unop in H4; destruct op in H4. 
-       inversion H4.
-       inversion h1; subst.
-       specialize (IHe (ValNormal (Bool b)) 0%Z b).
-       intuition.
-       rm_exists. 
-       specialize (eval_type_reserve s tb e (ValNormal (Bool b)) x h H2 H0); intros H8.
-       inversion H8; subst.
-       exists Tbool. rm_wt_expr.   
-    + (* well_defined *)
-       inversion h2 as [h3 | h4]; subst;
-       inversion h1; subst. 
-       unfold eval_unop in H4; destruct op in H4. 
-       inversion H4.
-       specialize (IHe (ValNormal (Bool b)) 0%Z b).
-       clear h2.
-       intuition.
-       rm_wd_expr.
-Qed.
-*)
+    + inversion H.
+       apply f_eval_expr_complete in H0. 
+       rewrite H0 in y.
+       destruct x in y; intuition.
 
 
 
-(* Prove the properties of the terminated program *)
-(*
-Theorem good_stmt_props: forall tb s s1 c,
-    symbol_consistent s tb /\ well_typed_stmt tb c /\ eval_stmt_R s c s1 ->
-        well_defined_stmt s c.
-Proof.
-    intros. inversion H; clear H. inversion H1; clear H1.
-    induction c.
-    (* 1. Sassign *)
-  - inversion H2; subst. 
-    eapply WD_Sassign.
-    inversion H; subst.
-    (* 2. Sifthen *)
- 
-    (* 3. Swhile *)
-  
-    (* 4. Sseq *)
-
-    (* 5. Sreturn *)
-  
-    (* 6. Sassert *)
-  
-    (* 7. Sloopinvariant *)
-
-*)
